lib/Language.ml
@@ -1,7 +1,6 @@
 open Specif
 
-module type Symbol =
- sig
+module type Symbol = sig
   type t
 
   val eq_dec : t -> t -> sumbool
@@ -11,4 +10,4 @@ module type Symbol =
   type string = t list
 
   val str_eq : string -> string -> sumbool
- end
+end
