lib/List.ml
@@ -1,7 +1,8 @@
-
 (** val list_prod : 'a1 list -> 'a2 list -> ('a1*'a2) list **)
 
 let rec list_prod l l' =
   match l with
-  | [] -> []
-  | x::t -> (@) (Stdlib.List.map (fun y -> x,y) l') (list_prod t l')
+  | [] ->
+      []
+  | x :: t ->
+      Stdlib.List.map (fun y -> (x, y)) l' @ list_prod t l'
