lib/Specif.ml
@@ -1,0 +1,8 @@
+type 'a coq_sig = 'a
+(* singleton inductive, whose constructor was exist *)
+
+type ('a, 'p) sigT = Coq_existT of 'a * 'p
+
+type sumbool = Coq_left | Coq_right
+
+type 'a sumor = Coq_inleft of 'a | Coq_inright
