lib/Teacher.ml
@@ -1,0 +1,25 @@
+open Lstar
+open Language
+
+module type Teacher = functor
+  (Coq_s : Symbol)
+  -> functor
+  (D : sig
+     type 'state t =
+       { transition: 'state -> Coq_s.t -> 'state
+       ; initial: 'state
+       ; accept: 'state -> bool }
+
+     val transition : 'a t -> 'a -> Coq_s.t -> 'a
+
+     val initial : 'a t -> 'a
+
+     val accept : 'a t -> 'a -> bool
+
+     val run : 'a t -> Coq_s.string -> 'a
+
+     val accept_string : 'a t -> Coq_s.string -> bool
+   end)
+  -> sig
+  val equiv_query : 'a D.t -> Coq_s.string option
+end
