theories/DFA.v
@@ -5,23 +5,22 @@ Module DFA (s : Symbol) (L : L s).
     Import s L.
 
     (** DFA type *)
-    Record t : Type := {
-        state : Type;
+    Record t (state : Type) : Type := {
         transition : state -> s.t -> state;
         initial : state;
         accept : state -> bool
     }.
 
     (** Run a DFA on a string and get the resulting state *)
-    Definition run (dfa : t) (s : string) : dfa.(state) :=
-        fold_left dfa.(transition) s dfa.(initial).
+    Definition run {state : Type} (dfa : t state) (s : string) : state :=
+        fold_left dfa.(transition state) s dfa.(initial state).
 
     (** Check whether a DFA reaches an accepting state after processing a string *)
-    Definition accept_string (dfa : t) (s : string) : bool :=
-        dfa.(accept) (run dfa s).
+    Definition accept_string {state : Type} (dfa : t state) (s : string) : bool :=
+        dfa.(accept state) (run dfa s).
 
     (** Whether a DFA encodes the language L *)
-    Definition encodes (dfa : t) : Prop :=
+    Definition encodes {state : Type} (dfa : t state) : Prop :=
         forall (s : string),
             member s = true <-> accept_string dfa s = true.
 End DFA.
