theories/Extraction.v
@@ -1,10 +1,10 @@
 From Stdlib Require Import Extraction.
 
-From lstar Require Import Lstar.
+From lstar Require Import Lstar DFA.
 
 Extraction Language OCaml.
 
-Set Extraction Output Directory "bin".
+Set Extraction Output Directory "lib".
 
 (* Uncomment to use some standard OCaml types for a small speedup *)
 From lstar Require Import ExtrOptimizations.
