README.md
@@ -3,7 +3,7 @@
 A formally-verified implementation of [Dana Angluin's L* algorithm](https://doi.org/10.1016/0890-5401(87)90052-6).
 The implementation is based on [these lecture notes](https://www.tifr.res.in/~shibashis.guha/courses/diwali2021/L-starMalharManagoli.pdf) and can be viewed [here](theories/Lstar.v).
 Functions return sigma types, so each sub-component of the algorithm provides a proof of correctness alongside its computational outputs.
-The extracted OCaml code can be seen [here](bin/Lstar.ml).
+The extracted OCaml code can be seen [here](lib/Lstar.ml).
 
 ## Building
 
