build.sh
@@ -1,11 +1,11 @@
 dune clean
 echo "[*] Building lstar-rocq"
 dune build -p lstar-rocq
-cp _build/default/bin/*.ml bin
-rm bin/Bin*.ml bin/PosDef.ml
+cp _build/default/lib/*.ml lib
+rm lib/Bin*.ml lib/PosDef.ml
 grep "^From lstar Require Import ExtrOptimizations" theories/Extraction.v > /dev/null
 if [ $? ]; then
-	rm bin/Bool.ml bin/ListDef.ml bin/PeanoNat.ml
+	rm lib/Bool.ml lib/ListDef.ml lib/PeanoNat.ml
 fi
 echo "[*] Building lstar"
 dune build -p lstar
